word range check func (#26)
* update

* update

* update

* update

* update

Test/CircuitTest.lean
@@ -73,8 +73,8 @@ def u8chip : Ast.Chip := {
 }
 
 @[simp]
-def wordRangeCheckerChip : Ast.Chip := {
-  name := "word_range_checker",
+def koalabearWordRangeCheckerChip : Ast.Chip := {
+  name := "koalabear_word_range_checker",
   ident_t := "trace",
   ident_i := "i",
   width := 18,
@@ -99,34 +99,22 @@ def wordRangeCheckerChip : Ast.Chip := {
           (.letIn "and_most_sig_byte_decomp_0_to_5" (Ast.trace_i_j "trace" "i" 15)
           (.letIn "and_most_sig_byte_decomp_0_to_6" (Ast.trace_i_j "trace" "i" 16)
           (.letIn "and_most_sig_byte_decomp_0_to_7" (Ast.trace_i_j "trace" "i" 17)
-          (.letIn "b₀" (.assertE (.fieldExpr (.var "most_sig_byte_decomp_0") .mul (.fieldExpr (.var "most_sig_byte_decomp_0") .sub (.constF 1))) (.constF 0))
-          (.letIn "b₁" (.assertE (.fieldExpr (.var "most_sig_byte_decomp_1") .mul (.fieldExpr (.var "most_sig_byte_decomp_1") .sub (.constF 1))) (.constF 0))
-          (.letIn "b₂" (.assertE (.fieldExpr (.var "most_sig_byte_decomp_2") .mul (.fieldExpr (.var "most_sig_byte_decomp_2") .sub (.constF 1))) (.constF 0))
-          (.letIn "b₃" (.assertE (.fieldExpr (.var "most_sig_byte_decomp_3") .mul (.fieldExpr (.var "most_sig_byte_decomp_3") .sub (.constF 1))) (.constF 0))
-          (.letIn "b₄" (.assertE (.fieldExpr (.var "most_sig_byte_decomp_4") .mul (.fieldExpr (.var "most_sig_byte_decomp_4") .sub (.constF 1))) (.constF 0))
-          (.letIn "b₅" (.assertE (.fieldExpr (.var "most_sig_byte_decomp_5") .mul (.fieldExpr (.var "most_sig_byte_decomp_5") .sub (.constF 1))) (.constF 0))
-          (.letIn "b₆" (.assertE (.fieldExpr (.var "most_sig_byte_decomp_6") .mul (.fieldExpr (.var "most_sig_byte_decomp_6") .sub (.constF 1))) (.constF 0))
-          (.letIn "b₇" (.assertE (.fieldExpr (.var "most_sig_byte_decomp_7") .mul (.fieldExpr (.var "most_sig_byte_decomp_7") .sub (.constF 1))) (.constF 0))
+          (.lookup "l₀" "u8" [(.var "value_0", (Ast.trace_i_j "trace" "i" 0))]
+          (.lookup "l₁" "u8" [(.var "value_1", (Ast.trace_i_j "trace" "i" 0))]
+          (.lookup "l₂" "u8" [(.var "value_2", (Ast.trace_i_j "trace" "i" 0))]
+          (.lookup "l₃" "u8" [(.var "value_3", (Ast.trace_i_j "trace" "i" 0))]
           (.letIn "u₁"
-            (.assertE (bits_to_byte_expr "most_sig_byte_decomp_0" "most_sig_byte_decomp_1" "most_sig_byte_decomp_2" "most_sig_byte_decomp_3"
-                                        "most_sig_byte_decomp_4" "most_sig_byte_decomp_5" "most_sig_byte_decomp_6" "most_sig_byte_decomp_7")
-              (.var "value_3")
-            )
-            (.letIn "u₂" (.assertE (.var "most_sig_byte_decomp_7") (.constF 0))
-            (.letIn "u₃" (.assertE (.var "and_most_sig_byte_decomp_0_to_2") (.fieldExpr (.var "most_sig_byte_decomp_0") .mul (.var "most_sig_byte_decomp_1")))
-            (.letIn "u₄" (.assertE (.var "and_most_sig_byte_decomp_0_to_3") (.fieldExpr (.var "and_most_sig_byte_decomp_0_to_2") .mul (.var "most_sig_byte_decomp_2")))
-            (.letIn "u₅" (.assertE (.var "and_most_sig_byte_decomp_0_to_4") (.fieldExpr (.var "and_most_sig_byte_decomp_0_to_3") .mul (.var "most_sig_byte_decomp_3")))
-            (.letIn "u₆" (.assertE (.var "and_most_sig_byte_decomp_0_to_5") (.fieldExpr (.var "and_most_sig_byte_decomp_0_to_4") .mul (.var "most_sig_byte_decomp_4")))
-            (.letIn "u₇" (.assertE (.var "and_most_sig_byte_decomp_0_to_6") (.fieldExpr (.var "and_most_sig_byte_decomp_0_to_5") .mul (.var "most_sig_byte_decomp_5")))
-            (.letIn "u₈" (.assertE (.var "and_most_sig_byte_decomp_0_to_7") (.fieldExpr (.var "and_most_sig_byte_decomp_0_to_6") .mul (.var "most_sig_byte_decomp_6")))
-            (.letIn "u₉" (.assertE (.constF 0) (.fieldExpr (.var "and_most_sig_byte_decomp_0_to_7") .mul (.var "value_0")))
-            (.letIn "u₁₀" (.assertE (.constF 0) (.fieldExpr (.var "and_most_sig_byte_decomp_0_to_7") .mul (.var "value_1")))
-            (.letIn "u₁₁" (.assertE (.constF 0) (.fieldExpr (.var "and_most_sig_byte_decomp_0_to_7") .mul (.var "value_2")))
-            (.lookup "l₀" "u8" [(.var "value_0", (Ast.trace_i_j "trace" "i" 0))]
-            (.lookup "l₁" "u8" [(.var "value_1", (Ast.trace_i_j "trace" "i" 0))]
-            (.lookup "l₂" "u8" [(.var "value_2", (Ast.trace_i_j "trace" "i" 0))]
-            (.lookup "l₃" "u8" [(.var "value_3", (Ast.trace_i_j "trace" "i" 0))]
-             (.var "l₃"))))))))))))))))))))))))))))))))))))))))))
+            (.app (.app (.app (.app (.app (.app (.app (.app (.app (.app (.app (.app (.app (.app (.app (.app (.app (.app
+              koalabear_word_range_checker_func
+                (.var "value_0")) (.var "value_1")) (.var "value_2")) (.var "value_3"))
+                (.var "most_sig_byte_decomp_0")) (.var "most_sig_byte_decomp_1"))
+                (.var "most_sig_byte_decomp_2")) (.var "most_sig_byte_decomp_3"))
+                (.var "most_sig_byte_decomp_4")) (.var "most_sig_byte_decomp_5"))
+                (.var "most_sig_byte_decomp_6")) (.var "most_sig_byte_decomp_7"))
+                (.var "and_most_sig_byte_decomp_0_to_2")) (.var "and_most_sig_byte_decomp_0_to_3"))
+                (.var "and_most_sig_byte_decomp_0_to_4")) (.var "and_most_sig_byte_decomp_0_to_5"))
+                (.var "and_most_sig_byte_decomp_0_to_6")) (.var "and_most_sig_byte_decomp_0_to_7"))
+            (.var "u₁"))))))))))))))))))))))))
 }
 
 def Δ : Env.ChipEnv := [("assert", assertChip), ("u8", u8chip)]
@@ -186,59 +174,38 @@ theorem iszeroChip2_correct : Ty.chipCorrect Δ iszeroChip2 1 := by
   simp
   apply lookup_update_self
   rfl
-  unfold Ast.renameTy
-  unfold Ast.renameVarinPred
-  unfold Ast.renameVar
-  simp
+  simp [Ast.renameTy, Ast.renameVarinPred, Ast.renameVar]
   apply Ty.TypeJudgment.TE_VarEnv
   apply lookup_update_ne_of_lookup
   simp
   apply lookup_update_self
   rfl
-  unfold Ast.renameTy
-  unfold Ast.renameVarinPred
-  unfold Ast.renameVar
-  simp
+  simp [Ast.renameTy, Ast.renameVarinPred, Ast.renameVar]
   apply Ty.TypeJudgment.TE_VarEnv
-  unfold Ast.renameVarinPred
-  simp
-  unfold Ast.renameVar
-  simp
   apply lookup_update_self
   rfl
-  unfold Ast.renameTy
-  unfold Ast.renameTy
-  unfold Ast.renameTy
-  unfold Ast.renameTy
-  simp
-  unfold Ast.renameVarinPred
-  unfold Ast.renameVarinPred
-  unfold Ast.renameVarinPred
-  simp
-  unfold Ast.renameVar
-  simp
-  unfold Ast.renameVar
-  simp
-  unfold Ast.renameVar
-  simp
-  unfold Ast.renameVar
-  simp
-  unfold Ast.renameVar
-  simp
-  unfold Ast.renameVar
-  simp
+  simp [Ast.renameTy, Ast.renameVarinPred, Ast.renameVar]
   apply Ty.TypeJudgment.TE_VarEnv
   apply lookup_update_self
 
-lemma lookup_u8_val_lt_256
-  (h₁: PropSemantics.tyenvToProp σ Δ Γ)
+lemma u8_lookup_refines_lt256 (u: String)
+  (h₁: @Ty.TypeJudgment Δ Γ Η (Ast.Expr.var x) (Ast.Ty.refin Ast.Ty.field Ast.constTruePred))
   (h₂: Env.lookupTy Γ u = some ((Ast.Ty.unit.refin
           (Ty.lookup_pred [(Ast.Expr.var x, Ast.trace_i_j "trace" "i" 0)] (Env.lookupChip Δ "u8")
             (Ast.Predicate.ind ((Ast.trace_i_j "trace" "i" 0).toZ.binRel Ast.RelOp.lt (Ast.Expr.constZ 256)))
             Η))))
   (h₃: (Env.freshName Η (Env.lookupChip Δ "u8").ident_i) = new_ident_i)
   (h₄: (Env.freshName Η (Env.lookupChip Δ "u8").ident_t) = new_ident_t)
-  (h₇: new_ident_t ≠ "i") :  ∃ v : F, Env.lookupVal σ x = some (Ast.Value.vF v) ∧ v.val < 256 := by {
+  (h₇: new_ident_t ≠ "i"):
+  @Ty.TypeJudgment Δ Γ Η (Ast.Expr.var x)
+    (Ast.Ty.refin Ast.Ty.field (Ast.Predicate.ind ((Ast.Expr.var x).toZ.binRel Ast.RelOp.lt (Ast.Expr.constZ 256))))
+  := by {
+    apply Ty.TypeJudgment.TE_SUB
+    apply h₁
+    apply Ty.SubtypeJudgment.TSub_Refine
+    apply Ty.SubtypeJudgment.TSub_Refl
+    intro σ' v h₈ h₉
+
     unfold Ty.lookup_pred at h₂
     have hu8_i : (Env.lookupChip Δ "u8").ident_i = "i" := by {
       unfold Env.lookupChip Δ
@@ -248,416 +215,102 @@ lemma lookup_u8_val_lt_256
       unfold Env.lookupChip Δ
       simp
     }
-
     rw[h₃, h₄, hu8_i, hu8_t] at h₂
-    unfold Ast.renameVarinPred Ast.renameVar at h₂
-    simp at h₂
-    unfold Ast.renameVarinPred Ast.renameVar at h₂
-    simp at h₂
-    unfold Ast.renameVar at h₂
-    simp at h₂
-    unfold Ast.renameVar at h₂
-    simp at h₂
-    unfold Ast.renameVar at h₂
-    simp at h₂
-    unfold Ast.renameVar at h₂
-    simp at h₂
+    simp [Ast.renameVarinPred, Ast.renameVar] at h₂
     rw [if_neg h₇] at h₂
-    have hl₀' := tyenv_and_to_eval_exprs h₁ h₂
 
-    obtain ⟨hl₀₁',hl₀₂'⟩ := hl₀'
-    have hvl₀ := eval_eq_then_lt hl₀₂' hl₀₁'
-    have hvl₀' := eval_lt_val hvl₀
-    exact hvl₀'
-  }
-
-lemma subtype_wordRange
-  (hb₁: Env.lookupTy Γ "b₀" = some (bit_value_type "most_sig_byte_decomp_0"))
-  (hb₂ : Env.lookupTy Γ "b₁" = some (bit_value_type "most_sig_byte_decomp_1"))
-  (hb₃: Env.lookupTy Γ "b₂" = some (bit_value_type "most_sig_byte_decomp_2"))
-  (hb₄ : Env.lookupTy Γ "b₃" = some (bit_value_type "most_sig_byte_decomp_3"))
-  (hb₅: Env.lookupTy Γ "b₄" = some (bit_value_type "most_sig_byte_decomp_4"))
-  (hb₆ : Env.lookupTy Γ "b₅" = some (bit_value_type "most_sig_byte_decomp_5"))
-  (hb₇: Env.lookupTy Γ "b₆" = some (bit_value_type "most_sig_byte_decomp_6"))
-  (hb₈ : Env.lookupTy Γ "b₇" = some (bit_value_type "most_sig_byte_decomp_7"))
-  (hu₁: Env.lookupTy Γ "u₁" = some (Ast.Ty.unit.refin
-                                  (Ast.Predicate.ind
-                                    (Ast.exprEq
-                                      (bits_to_byte_expr "most_sig_byte_decomp_0" "most_sig_byte_decomp_1" "most_sig_byte_decomp_2" "most_sig_byte_decomp_3"
-                                                        "most_sig_byte_decomp_4" "most_sig_byte_decomp_5" "most_sig_byte_decomp_6" "most_sig_byte_decomp_7")
-                                      (Ast.Expr.var "value_3")))))
-  (hu₂: Env.lookupTy Γ "u₂" = some                               (Ast.Ty.unit.refin
-                                (Ast.Predicate.ind
-                                  (Ast.exprEq (Ast.Expr.var "most_sig_byte_decomp_7") (Ast.Expr.constF 0)))))
-  (hu₃: Env.lookupTy Γ "u₃" = some (eq_mul_refinement "and_most_sig_byte_decomp_0_to_2" "most_sig_byte_decomp_0" "most_sig_byte_decomp_1"))
-  (hu₄: Env.lookupTy Γ "u₄" = some (eq_mul_refinement "and_most_sig_byte_decomp_0_to_3" "and_most_sig_byte_decomp_0_to_2" "most_sig_byte_decomp_2"))
-  (hu₅: Env.lookupTy Γ "u₅" = some (eq_mul_refinement "and_most_sig_byte_decomp_0_to_4" "and_most_sig_byte_decomp_0_to_3" "most_sig_byte_decomp_3"))
-  (hu₆: Env.lookupTy Γ "u₆" = some (eq_mul_refinement "and_most_sig_byte_decomp_0_to_5" "and_most_sig_byte_decomp_0_to_4" "most_sig_byte_decomp_4"))
-  (hu₇: Env.lookupTy Γ "u₇" = some (eq_mul_refinement "and_most_sig_byte_decomp_0_to_6" "and_most_sig_byte_decomp_0_to_5" "most_sig_byte_decomp_5"))
-  (hu₈: Env.lookupTy Γ "u₈" = some (eq_mul_refinement "and_most_sig_byte_decomp_0_to_7" "and_most_sig_byte_decomp_0_to_6" "most_sig_byte_decomp_6"))
-  (hu₉: Env.lookupTy Γ "u₉" = some                           (Ast.Ty.unit.refin
-                  (Ast.Predicate.ind
-                    (Ast.exprEq (Ast.Expr.constF 0)
-                      ((Ast.Expr.var "and_most_sig_byte_decomp_0_to_7").fieldExpr Ast.FieldOp.mul
-                        (Ast.Expr.var "value_0"))))))
-  (hu₁₀: Env.lookupTy Γ "u₁₀" = some                           (Ast.Ty.unit.refin
-                (Ast.Predicate.ind
-                  (Ast.exprEq (Ast.Expr.constF 0)
-                    ((Ast.Expr.var "and_most_sig_byte_decomp_0_to_7").fieldExpr Ast.FieldOp.mul
-                      (Ast.Expr.var "value_1"))))))
-  (hu₁₁: Env.lookupTy Γ "u₁₁" = some                           (Ast.Ty.unit.refin
-                (Ast.Predicate.ind
-                  (Ast.exprEq (Ast.Expr.constF 0)
-                    ((Ast.Expr.var "and_most_sig_byte_decomp_0_to_7").fieldExpr Ast.FieldOp.mul
-                      (Ast.Expr.var "value_2"))))))
-  ( hl₀ : Env.lookupTy Γ "l₀" = some ((Ast.Ty.unit.refin
-            (Ty.lookup_pred [(Ast.Expr.var "value_0", Ast.trace_i_j "trace" "i" 0)] (Env.lookupChip Δ "u8")
-              (Ast.Predicate.ind ((Ast.trace_i_j "trace" "i" 0).toZ.binRel Ast.RelOp.lt (Ast.Expr.constZ 256)))
-              [wordRangeCheckerChip.ident_i, wordRangeCheckerChip.ident_t]))))
-  ( hl₁: Env.lookupTy Γ "l₁" = some (        (Ast.Ty.unit.refin
-          (Ty.lookup_pred [(Ast.Expr.var "value_1", Ast.trace_i_j "trace" "i" 0)] (Env.lookupChip Δ "u8")
-            (Ast.Predicate.ind ((Ast.trace_i_j "trace" "i" 0).toZ.binRel Ast.RelOp.lt (Ast.Expr.constZ 256)))
-            (Ty.update_UsedNames (Env.lookupChip Δ "u8")
-              [wordRangeCheckerChip.ident_i, wordRangeCheckerChip.ident_t])))))
-  ( hl₂: Env.lookupTy Γ "l₂" =       (Ast.Ty.unit.refin
-        (Ty.lookup_pred [(Ast.Expr.var "value_2", Ast.trace_i_j "trace" "i" 0)] (Env.lookupChip Δ "u8")
-          (Ast.Predicate.ind ((Ast.trace_i_j "trace" "i" 0).toZ.binRel Ast.RelOp.lt (Ast.Expr.constZ 256)))
-          (Ty.update_UsedNames (Env.lookupChip Δ "u8")
-            (Ty.update_UsedNames (Env.lookupChip Δ "u8")
-              [wordRangeCheckerChip.ident_i, wordRangeCheckerChip.ident_t])))))
-  ( hl₃: Env.lookupTy Γ "l₃" = (Ast.Ty.unit.refin
-      (Ty.lookup_pred [(Ast.Expr.var "value_3", Ast.trace_i_j "trace" "i" 0)] (Env.lookupChip Δ "u8")
-        (Ast.Predicate.ind ((Ast.trace_i_j "trace" "i" 0).toZ.binRel Ast.RelOp.lt (Ast.Expr.constZ 256)))
-        (Ty.update_UsedNames (Env.lookupChip Δ "u8")
-          (Ty.update_UsedNames (Env.lookupChip Δ "u8")
-            (Ty.update_UsedNames (Env.lookupChip Δ "u8")
-              [wordRangeCheckerChip.ident_i, wordRangeCheckerChip.ident_t]))))))
-  : @Ty.SubtypeJudgment Δ Γ (Ast.Ty.unit.refin
-      (Ty.lookup_pred [(Ast.Expr.var "value_3", Ast.trace_i_j "trace" "i" 0)] (Env.lookupChip Δ "u8")
-        (Ast.Predicate.ind ((Ast.trace_i_j "trace" "i" 0).toZ.binRel Ast.RelOp.lt (Ast.Expr.constZ 256)))
-        (Ty.update_UsedNames (Env.lookupChip Δ "u8")
-          (Ty.update_UsedNames (Env.lookupChip Δ "u8")
-            (Ty.update_UsedNames (Env.lookupChip Δ "u8")
-              [wordRangeCheckerChip.ident_i, wordRangeCheckerChip.ident_t]))))) wordRangeCheckerChip.goal := by {
-    apply Ty.SubtypeJudgment.TSub_Refine
-    apply Ty.SubtypeJudgment.TSub_Refl
-    intro σ v h₁ h₂
-
-    have hb₁' := tyenv_to_eval_expr h₁ hb₁
-    have hb₂' := tyenv_to_eval_expr h₁ hb₂
-    have hb₃' := tyenv_to_eval_expr h₁ hb₃
-    have hb₄' := tyenv_to_eval_expr h₁ hb₄
-    have hb₅' := tyenv_to_eval_expr h₁ hb₅
-    have hb₆' := tyenv_to_eval_expr h₁ hb₆
-    have hb₇' := tyenv_to_eval_expr h₁ hb₇
-    have hb₈' := tyenv_to_eval_expr h₁ hb₈
-    have hu₁' := tyenv_to_eval_expr h₁ hu₁
-    have hu₂' := tyenv_to_eval_expr h₁ hu₂
-    have hu₃' := tyenv_to_eval_expr h₁ hu₃
-    have hu₄' := tyenv_to_eval_expr h₁ hu₄
-    have hu₅' := tyenv_to_eval_expr h₁ hu₅
-    have hu₆' := tyenv_to_eval_expr h₁ hu₆
-    have hu₇' := tyenv_to_eval_expr h₁ hu₇
-    have hu₈' := tyenv_to_eval_expr h₁ hu₈
-    have hu₉' := tyenv_to_eval_expr h₁ hu₉
-    have hu₁₀' := tyenv_to_eval_expr h₁ hu₁₀
-    have hu₁₁' := tyenv_to_eval_expr h₁ hu₁₁
-    have hb₁'' := eval_bit_expr_val hb₁'
-    have hb₂'' := eval_bit_expr_val hb₂'
-    have hb₃'' := eval_bit_expr_val hb₃'
-    have hb₄'' := eval_bit_expr_val hb₄'
-    have hb₅'' := eval_bit_expr_val hb₅'
-    have hb₆'' := eval_bit_expr_val hb₆'
-    have hb₇'' := eval_bit_expr_val hb₇'
-    have hb₈'' := eval_bit_expr_val hb₈'
-    have hu₁' := eval_bits_to_byte_expr_val hu₁'
-    have hu₃'' := eval_mul_expr_val hu₃'
-    have hu₄'' := eval_mul_expr_val hu₄'
-    have hu₅'' := eval_mul_expr_val hu₅'
-    have hu₆'' := eval_mul_expr_val hu₆'
-    have hu₇'' := eval_mul_expr_val hu₇'
-    have hu₈'' := eval_mul_expr_val hu₈'
-    have hu₉'' := eval_eq_const_mul_val hu₉'
-    have hu₁₀'' := eval_eq_const_mul_val hu₁₀'
-    have hu₁₁'' := eval_eq_const_mul_val hu₁₁'
-
-    cases hu₂'
-    rename_i v₁ u₁ ih₁ ih₂ h_most_sig_byte_decomp_7_is_0
-    cases ih₁
-    cases ih₂
-    unfold Eval.evalRelOp at h_most_sig_byte_decomp_7_is_0
-    cases v₁ <;> simp at h_most_sig_byte_decomp_7_is_0
-    rename_i most_sig_byte_decomp_7 h_most_sig_byte_decomp_7_env
-
-    have hu8_i : (Env.lookupChip Δ "u8").ident_i = "i" := by {
-      unfold Env.lookupChip Δ
-      simp
-    }
-    have hu8_t : (Env.lookupChip Δ "u8").ident_t = "trace" := by {
-      unfold Env.lookupChip Δ
-      simp
-    }
-    have h₁' : (Env.freshName [wordRangeCheckerChip.ident_i, wordRangeCheckerChip.ident_t] (Env.lookupChip Δ "u8").ident_t) = "trace'" := by {
-      unfold Env.freshName
-      rw[hu8_t]
-      simp
-    }
-    have h₂' : (Env.freshName [wordRangeCheckerChip.ident_i, wordRangeCheckerChip.ident_t] (Env.lookupChip Δ "u8").ident_i) = "i'" := by {
-      unfold Env.freshName
-      rw[hu8_i]
-      simp
-    }
-    have h₃' : "trace'" ≠ "i" := by simp
-    have hl₀' := tyenv_and_to_eval_exprs h₁ hl₀
-    have hvl₀ := lookup_u8_val_lt_256 h₁ hl₀ h₂' h₁' h₃'
-    have h₁' : (Env.freshName (Ty.update_UsedNames (Env.lookupChip Δ "u8")
-              [wordRangeCheckerChip.ident_i, wordRangeCheckerChip.ident_t]) (Env.lookupChip Δ "u8").ident_t) = "trace'" := by {
-      unfold Env.freshName
-      rw[hu8_t]
-      simp
-      unfold Ty.update_UsedNames
-      simp
-    }
-    have h₂' : (Env.freshName (Ty.update_UsedNames (Env.lookupChip Δ "u8")
-              [wordRangeCheckerChip.ident_i, wordRangeCheckerChip.ident_t]) (Env.lookupChip Δ "u8").ident_i) = "i'" := by {
-      unfold Env.freshName
-      rw[hu8_i]
-      simp
-      unfold Ty.update_UsedNames
-      simp
-    }
-    have hl₁' := tyenv_and_to_eval_exprs h₁ hl₁
-    have hvl₁ := lookup_u8_val_lt_256 h₁ hl₁ h₂' h₁' h₃'
-    have h₁' : (Env.freshName (Ty.update_UsedNames (Env.lookupChip Δ "u8")
-          (Ty.update_UsedNames (Env.lookupChip Δ "u8")
-            (Ty.update_UsedNames (Env.lookupChip Δ "u8")
-              [wordRangeCheckerChip.ident_i, wordRangeCheckerChip.ident_t]))) (Env.lookupChip Δ "u8").ident_t) = "trace'" := by {
-      unfold Env.freshName
-      rw[hu8_t]
-      simp
-      unfold Ty.update_UsedNames
-      simp
-    }
-    have h₂' : (Env.freshName (Ty.update_UsedNames (Env.lookupChip Δ "u8")
-          (Ty.update_UsedNames (Env.lookupChip Δ "u8")
-            (Ty.update_UsedNames (Env.lookupChip Δ "u8")
-              [wordRangeCheckerChip.ident_i, wordRangeCheckerChip.ident_t]))) (Env.lookupChip Δ "u8").ident_i) = "i'" := by {
-      unfold Env.freshName
-      rw[hu8_i]
-      simp
-      unfold Ty.update_UsedNames
-      simp
-    }
-    have hl₂' := tyenv_and_to_eval_exprs h₁ hl₂
-    have hvl₂ := lookup_u8_val_lt_256 h₁ hl₂ h₂' h₁' h₃'
-    have hl₃' := tyenv_and_to_eval_exprs h₁ hl₃
-    have hvl₃ := lookup_u8_val_lt_256 h₁ hl₃ h₂' h₁' h₃'
+    have he := tyenv_and_to_eval_exprs h₈ h₂
+    obtain ⟨he₁,he₂⟩ := he
+    have he₃ := eval_eq_then_lt he₂ he₁
 
     unfold PropSemantics.predToProp PropSemantics.exprToProp
-    obtain ⟨most_sig_byte_decomp_0, h⟩ := hb₁''
-    obtain ⟨h_most_sig_byte_decomp_0_env, h_most_sig_byte_decomp_0⟩ := h
-    obtain ⟨most_sig_byte_decomp_1, h⟩ := hb₂''
-    obtain ⟨h_most_sig_byte_decomp_1_env, h_most_sig_byte_decomp_1⟩ := h
-    obtain ⟨most_sig_byte_decomp_2, h⟩ := hb₃''
-    obtain ⟨h_most_sig_byte_decomp_2_env, h_most_sig_byte_decomp_2⟩ := h
-    obtain ⟨most_sig_byte_decomp_3, h⟩ := hb₄''
-    obtain ⟨h_most_sig_byte_decomp_3_env, h_most_sig_byte_decomp_3⟩ := h
-    obtain ⟨most_sig_byte_decomp_4, h⟩ := hb₅''
-    obtain ⟨h_most_sig_byte_decomp_4_env, h_most_sig_byte_decomp_4⟩ := h
-    obtain ⟨most_sig_byte_decomp_5, h⟩ := hb₆''
-    obtain ⟨h_most_sig_byte_decomp_5_env, h_most_sig_byte_decomp_5⟩ := h
-    obtain ⟨most_sig_byte_decomp_6, h⟩ := hb₇''
-    obtain ⟨h_most_sig_byte_decomp_6_env, h_most_sig_byte_decomp_6⟩ := h
-    obtain ⟨most_sig_byte_decomp_7', h⟩ := hb₈''
-    obtain ⟨h_most_sig_byte_decomp_7_env', h_most_sig_byte_decomp_7⟩ := h
-    rw[h_most_sig_byte_decomp_7_env] at h_most_sig_byte_decomp_7_env'
-    simp at h_most_sig_byte_decomp_7_env'
-    rw[← h_most_sig_byte_decomp_7_env'] at h_most_sig_byte_decomp_7
+    exact he₃
+  }
 
-    obtain ⟨v₀, v₁, v₂, v₃, v₄, v₅, v₆, v₇, value_3, h⟩ := hu₁'
-    obtain ⟨h₁, h₂, h₃, h₄, h₅, h₆, h₇, h₈, h_value_3_env, h_msb_rec⟩ := h
-    simp at h_most_sig_byte_decomp_0_env h_most_sig_byte_decomp_1_env
-            h_most_sig_byte_decomp_2_env h_most_sig_byte_decomp_3_env
-            h_most_sig_byte_decomp_4_env h_most_sig_byte_decomp_5_env
-            h_most_sig_byte_decomp_6_env h_most_sig_byte_decomp_7_env
-    rw[h_most_sig_byte_decomp_0_env] at h₁
-    rw[h_most_sig_byte_decomp_1_env] at h₂
-    rw[h_most_sig_byte_decomp_2_env] at h₃
-    rw[h_most_sig_byte_decomp_3_env] at h₄
-    rw[h_most_sig_byte_decomp_4_env] at h₅
-    rw[h_most_sig_byte_decomp_5_env] at h₆
-    rw[h_most_sig_byte_decomp_6_env] at h₇
-    rw[h_most_sig_byte_decomp_7_env] at h₈
-    simp at h₁ h₂ h₃ h₄ h₅ h₆ h₇ h₈ h_value_3_env
-    rw[← h₁, ← h₂, ← h₃, ← h₄, ← h₅, ← h₆, ← h₇, ← h₈] at h_msb_rec
+lemma u8_freshName_ne_i : Env.freshName
+    (Ty.update_UsedNames (Env.lookupChip Δ "u8")
+      (Ty.update_UsedNames (Env.lookupChip Δ "u8")
+        (Ty.update_UsedNames (Env.lookupChip Δ "u8")
+          (Ty.update_UsedNames (Env.lookupChip Δ "u8") ["i", "trace"]))))
+    (Env.lookupChip Δ "u8").ident_t ≠
+  "i" := by {
+    unfold Ty.update_UsedNames Env.lookupChip Δ
+    simp [Env.freshName]
+  }
 
-    obtain ⟨and_most_sig_byte_decomp_0_to_2, v₂, v₃, h⟩ := hu₃''
-    obtain ⟨h_and_most_sig_byte_decomp_0_to_2_env, h₂, h₃, hamm₁⟩ := h
-    simp at h_and_most_sig_byte_decomp_0_to_2_env h₂ h₃ hamm₁
-    rw[h_most_sig_byte_decomp_0_env] at h₂
-    rw[h_most_sig_byte_decomp_1_env] at h₃
-    simp at h₂ h₃ hamm₁
-    rw[← h₂, ← h₃] at hamm₁
-
-
-    obtain ⟨and_most_sig_byte_decomp_0_to_3, v₂, v₃, h⟩ := hu₄''
-    obtain ⟨h_and_most_sig_byte_decomp_0_to_3_env, h₂, h₃, hamm₂⟩ := h
-    simp at h_and_most_sig_byte_decomp_0_to_3_env h₂ h₃ hamm₂
-    rw[h_and_most_sig_byte_decomp_0_to_2_env] at h₂
-    rw[h_most_sig_byte_decomp_2_env] at h₃
-    simp at h₂ h₃ hamm₂
-    rw[← h₂, ← h₃] at hamm₂
-
-    obtain ⟨and_most_sig_byte_decomp_0_to_4, v₂, v₃, h⟩ := hu₅''
-    obtain ⟨h_and_most_sig_byte_decomp_0_to_4_env, h₂, h₃, hamm₃⟩ := h
-    simp at h_and_most_sig_byte_decomp_0_to_4_env h₂ h₃ hamm₃
-    rw[h_and_most_sig_byte_decomp_0_to_3_env] at h₂
-    rw[h_most_sig_byte_decomp_3_env] at h₃
-    simp at h₂ h₃ hamm₃
-    rw[← h₂, ← h₃] at hamm₃
-
-    obtain ⟨and_most_sig_byte_decomp_0_to_5, v₂, v₃, h⟩ := hu₆''
-    obtain ⟨h_and_most_sig_byte_decomp_0_to_5_env, h₂, h₃, hamm₄⟩ := h
-    simp at h_and_most_sig_byte_decomp_0_to_5_env h₂ h₃ hamm₄
-    rw[h_and_most_sig_byte_decomp_0_to_4_env] at h₂
-    rw[h_most_sig_byte_decomp_4_env] at h₃
-    simp at h₂ h₃ hamm₄
-    rw[← h₂, ← h₃] at hamm₄
-
-    obtain ⟨and_most_sig_byte_decomp_0_to_6, v₂, v₃, h⟩ := hu₇''
-    obtain ⟨h_and_most_sig_byte_decomp_0_to_6_env, h₂, h₃, hamm₅⟩ := h
-    simp at h_and_most_sig_byte_decomp_0_to_6_env h₂ h₃ hamm₅
-    rw[h_and_most_sig_byte_decomp_0_to_5_env] at h₂
-    rw[h_most_sig_byte_decomp_5_env] at h₃
-    simp at h₂ h₃ hamm₅
-    rw[← h₂, ← h₃] at hamm₅
-
-    obtain ⟨and_most_sig_byte_decomp_0_to_7, v₂, v₃, h⟩ := hu₈''
-    obtain ⟨h_and_most_sig_byte_decomp_0_to_7_env, h₂, h₃, hamm₆⟩ := h
-    simp at h_and_most_sig_byte_decomp_0_to_7_env h₂ h₃ hamm₆
-    rw[h_and_most_sig_byte_decomp_0_to_6_env] at h₂
-    rw[h_most_sig_byte_decomp_6_env] at h₃
-    simp at h₂ h₃ hamm₆
-    rw[← h₂, ← h₃] at hamm₆
-
-    obtain ⟨v₁, value_0, h⟩ := hu₉''
-    obtain ⟨h₁, h_value_0_env, hav₀⟩ := h
-    simp at h₁ h_value_0_env hav₀
-    rw[h_and_most_sig_byte_decomp_0_to_7_env] at h₁
-    simp at h₁
-    rw[← h₁] at hav₀
-
-
-    obtain ⟨v₁, value_1, h⟩ := hu₁₀''
-    obtain ⟨h₁, h_value_1_env, hav₁⟩ := h
-    simp at h₁ h_value_1_env hav₁
-    rw[h_and_most_sig_byte_decomp_0_to_7_env] at h₁
-    simp at h₁
-    rw[← h₁] at hav₁
-
-    obtain ⟨v₁, value_2, h⟩ := hu₁₁''
-    obtain ⟨h₁, h_value_2_env, hav₂⟩ := h
-    simp at h₁ h_value_2_env hav₂
-    rw[h_and_most_sig_byte_decomp_0_to_7_env] at h₁
-    simp at h₁
-    rw[← h₁] at hav₂
-
-    obtain ⟨v₁, h₁, hvl₀⟩ := hvl₀
-    simp at h₁
-    rw[h_value_0_env] at h₁
-    simp at h₁
-    rw[← h₁] at hvl₀
-
-    obtain ⟨v₁, h₁, hvl₁⟩ := hvl₁
-    simp at h₁
-    rw[h_value_1_env] at h₁
-    simp at h₁
-    rw[← h₁] at hvl₁
-
-    obtain ⟨v₁, h₁, hvl₂⟩ := hvl₂
-    simp at h₁
-    rw[h_value_2_env] at h₁
-    simp at h₁
-    rw[← h₁] at hvl₂
-
-    obtain ⟨v₁, h₁, hvl₃⟩ := hvl₃
-    simp at h₁
-    rw[h_value_3_env] at h₁
-    simp at h₁
-    rw[← h₁] at hvl₃
-
-    repeat
-      repeat constructor
-      assumption
-    repeat constructor
-    simp
-    apply word32_range_under_koalabear
-      (bit_value_mul_zero h_most_sig_byte_decomp_0) (bit_value_mul_zero h_most_sig_byte_decomp_1)
-      (bit_value_mul_zero h_most_sig_byte_decomp_2) (bit_value_mul_zero h_most_sig_byte_decomp_3)
-      (bit_value_mul_zero h_most_sig_byte_decomp_4) (bit_value_mul_zero h_most_sig_byte_decomp_5)
-      (bit_value_mul_zero h_most_sig_byte_decomp_6) (bit_value_mul_zero h_most_sig_byte_decomp_7)
-      h_msb_rec h_most_sig_byte_decomp_7_is_0 hamm₁ hamm₂ hamm₃ hamm₄ hamm₅ hamm₆
-    simp
-    exact hav₀
-    simp
-    exact hav₁
-    simp
-    repeat assumption
-}
-
-
-theorem wordRangeCheckerChip_correct : Ty.chipCorrect Δ wordRangeCheckerChip 1 := by
+theorem koalabearWordRangeCheckerChip_correct : Ty.chipCorrect Δ koalabearWordRangeCheckerChip 1 := by
   unfold Ty.chipCorrect
   intro x i hs hi hrow ht hσ
   let envs := Ty.makeEnvs assertChip (Ast.Value.vArr x) (Ast.Value.vZ i) x.length
   let σ := envs.1
   let Γ := envs.2
   auto_trace_index
+  repeat
+    apply Ty.TypeJudgment.TE_LookUp
+    rfl; rfl; rfl
   apply Ty.TypeJudgment.TE_LetIn
-  · apply lookup_update_self;
-  . apply Ty.TypeJudgment.TE_Assert
-    repeat
-      apply Ty.TypeJudgment.TE_BinOpField
-    auto_resolve_varenv
-    apply Ty.TypeJudgment.TE_BinOpField
-    auto_resolve_varenv
-    repeat apply Ty.TypeJudgment.TE_ConstF
-  . repeat
-      auto_let_assert
-      repeat
-        apply Ty.TypeJudgment.TE_BinOpField
-        auto_resolve_varenv
-      apply Ty.TypeJudgment.TE_ConstF
-      apply Ty.TypeJudgment.TE_ConstF
-    auto_let_assert
-    repeat apply Ty.TypeJudgment.TE_BinOpField
-    auto_resolve_varenv
-    repeat
-      apply Ty.TypeJudgment.TE_BinOpField
-      auto_resolve_varenv
-      apply Ty.TypeJudgment.TE_ConstF
-    auto_resolve_varenv
-    auto_let_assert
-    auto_resolve_varenv
-    apply Ty.TypeJudgment.TE_ConstF
-    repeat
-      auto_let_assert
-      auto_resolve_varenv
-      apply Ty.TypeJudgment.TE_BinOpField
-      repeat auto_resolve_varenv
-    repeat
-      auto_let_assert
-      apply Ty.TypeJudgment.TE_ConstF
-      apply Ty.TypeJudgment.TE_BinOpField
-      repeat auto_resolve_varenv
-    repeat
-      apply Ty.TypeJudgment.TE_LookUp
-      rfl; rfl; rfl
-    apply Ty.TypeJudgment.TE_SUB
+  apply lookup_update_self
+  repeat apply Ty.TypeJudgment.TE_App
+  apply koalabear_word_range_checker_func_typing_soundness
+  apply u8_lookup_refines_lt256 "l₀"
+  apply Ty.TypeJudgment.TE_VarEnv
+  apply lookup_update_ne
+  simp
+  repeat rfl
+  exact u8_freshName_ne_i
+  rfl
+  simp [Ast.renameTy, Ast.renameVarinPred, Ast.renameVar]
+  apply u8_lookup_refines_lt256 "l₁"
+  apply Ty.TypeJudgment.TE_VarEnv
+  apply lookup_update_ne
+  simp
+  repeat rfl
+  exact u8_freshName_ne_i
+  rfl
+  simp [Ast.renameTy, Ast.renameVarinPred, Ast.renameVar]
+  apply u8_lookup_refines_lt256 "l₂"
+  apply Ty.TypeJudgment.TE_VarEnv
+  apply lookup_update_ne
+  simp
+  repeat rfl
+  exact u8_freshName_ne_i
+  rfl
+  simp [Ast.renameTy, Ast.renameVarinPred, Ast.renameVar]
+  apply u8_lookup_refines_lt256 "l₃"
+  apply Ty.TypeJudgment.TE_VarEnv
+  apply lookup_update_ne
+  simp
+  repeat rfl
+  exact u8_freshName_ne_i
+  rfl
+  simp [Ast.renameTy, Ast.renameVarinPred, Ast.renameVar]
+  apply Ty.TypeJudgment.TE_VarEnv
+  apply lookup_update_ne
+  simp
+  rfl
+  apply Ty.TypeJudgment.TE_VarEnv
+  simp [Ast.renameVarinPred, Ast.renameVar]
+  apply lookup_update_ne
+  simp
+  simp [Ast.renameTy, Ast.renameVarinPred, Ast.renameVar]
+  apply And.intro
+  rfl
+  apply And.intro
+  repeat rfl
+  repeat
     apply Ty.TypeJudgment.TE_VarEnv
-    apply lookup_update_self
-    apply subtype_wordRange
-    repeat
-      apply lookup_update_ne
-      simp
-    apply lookup_update_self
+    apply lookup_update_ne
+    simp
+    simp [Ast.renameTy, Ast.renameVarinPred, Ast.renameVar]
+    apply And.intro
+    rfl
+    apply And.intro
+    rfl
+    rfl
+  apply Ty.TypeJudgment.TE_VarEnv
+  apply lookup_update_ne
+  simp
+  simp [Ast.renameTy, Ast.renameVarinPred, Ast.renameVar]
+  rfl
+  apply Ty.TypeJudgment.TE_VarEnv
+  apply lookup_update_self
